src/simple-proof/proof/OperationalSemantics.v
@@ -13,7 +13,7 @@ Inductive red : sta * trm -> sta * trm -> Prop :=
     [―――――――――――――――――――――――――]  #<br>#
     [(s, x.a) |-> (s, t)      ]  *)
 | red_sel : forall x m s t T ds,
-    binds x (val_new T ds) s ->
+    binds x (val_obj T ds) s ->
     defs_has (open_defs x ds) (def_trm m t) ->
     (s, trm_sel (avar_f x) m) |-> (s, t)
 
@@ -21,7 +21,7 @@ Inductive red : sta * trm -> sta * trm -> Prop :=
     [―――――――――――――――――――――]  #<br>#
     [(s, x y) |-> (s, t^y)]  *)
 | red_app : forall f a s T t,
-    binds f (val_lambda T t) s ->
+    binds f (val_fun T t) s ->
     (s, trm_app (avar_f f) (avar_f a)) |-> (s, open_trm a t)
 
 (** [(s, let x = v in t) |-> ((s, x = v), t^x)] *)
